examples/pseudo_bool/pb_checkProgScript.sml
@@ -1,0 +1,221 @@
+(*
+  This produces an executable program for pb_check
+*)
+open preamble basis pb_checkTheory;
+
+val _ = new_theory "pb_checkProg"
+
+val _ = translation_extends"basisProg";
+
+Definition noparse_string_def:
+  noparse_string f s = concat[strlit"c Input file: ";f;strlit" unable to parse in format: "; s;strlit"\n"]
+End
+
+val r = translate noparse_string_def;
+
+Definition usage_string_def:
+  usage_string = strlit "Usage:  cake_pb <OPB format formula file> <Proof file>\n"
+End
+
+val r = translate usage_string_def;
+
+Definition notfound_string_def:
+  notfound_string f = concat[strlit"c Input file: ";f;strlit" no such file or directory\n"]
+End
+
+val r = translate notfound_string_def;
+
+(* translation for .pbf parsing *)
+val r = translate blanks_def;
+val r = translate tokenize_def;
+val r = translate nocomment_line_def;
+
+val r = translate parse_lit_def;
+
+val parse_lit_side_def = definition"parse_lit_side_def";
+val parse_lit_side = Q.prove(
+  `∀x. parse_lit_side x <=> T`,
+  rw[parse_lit_side_def])
+  |> update_precondition;
+
+val r = translate parse_constraint_LHS_def;
+val r = translate strip_terminator_def;
+
+val strip_terminator_side_def = definition"strip_terminator_side_def";
+val strip_terminator_side = Q.prove(
+  `∀x. strip_terminator_side x <=> T`,
+  rw[strip_terminator_side_def])
+  |> update_precondition;
+
+val r = translate add_terms_denorm_def;
+val r = translate pb_constraintTheory.get_var_def;
+val r = translate term_eq_def;
+val r = translate merge_adjacent_def;
+val r = translate pb_constraintTheory.negate_def;
+val r = translate normalize_def;
+
+val normalize_side_def = theorem"normalize_side_def";
+val normalize_side = Q.prove(
+  `∀x y z. normalize_side x y z <=> T`,
+  Induct>>rw[Once normalize_side_def]>>
+  intLib.ARITH_TAC) |> update_precondition;
+
+val r = translate term_le_def;
+val r = translate normalize_PBC_def;
+
+val normalize_pbc_side = Q.prove(
+  `∀x y. normalize_pbc_side x y <=> T`,
+  EVAL_TAC>>rw[]>>
+  intLib.ARITH_TAC) |> update_precondition;
+
+val r = translate parse_constraint_def;
+val r = translate parse_constraints_def;
+
+val r = translate parse_pbf_toks_def;
+
+val parse_pbf_full = (append_prog o process_topdecs) `
+  fun parse_pbf_full f =
+  (case TextIO.b_inputAllTokensFrom f blanks tokenize of
+    None => Inl (notfound_string f)
+  | Some lines =>
+  (case parse_pbf_toks lines of
+    None => Inl (noparse_string f "OPB")
+  | Some x => Inr x))`
+
+val r = translate tokenize_num_def;
+val r = translate strip_numbers_def;
+val r = translate parse_polish_def;
+val r = translate parse_pbpstep_def;
+val r = translate parse_pbpsteps_def;
+val r = translate parse_pbp_toks_def;
+
+val parse_pbp_full = (append_prog o process_topdecs) `
+  fun parse_pbp_full f =
+  (case TextIO.b_inputAllTokensFrom f blanks tokenize_num of
+    None => Inl (notfound_string f)
+  | Some lines =>
+  (case parse_pbp_toks lines of
+    None => Inl (noparse_string f "PBP")
+  | Some x => Inr x))`
+
+val r = translate insert_def;
+val r = translate lookup_def;
+val r = translate mk_BN_def;
+val r = translate mk_BS_def;
+val r = translate delete_def;
+val r = translate build_fml_def;
+
+val r = translate (lslack_def |> SIMP_RULE std_ss [MEMBER_INTRO]);
+val r = translate (check_contradiction_def |> SIMP_RULE std_ss[LET_DEF]);
+
+(* add *)
+val r = translate pb_constraintTheory.term_lt_def;
+val r = translate pb_constraintTheory.add_terms_def;
+val r = translate pb_constraintTheory.add_lists_def;
+val r = translate pb_constraintTheory.add_def;
+
+val r = translate pb_constraintTheory.multiply_def;
+val r = translate pb_constraintTheory.div_ceiling_def;
+val r = translate pb_constraintTheory.divide_def;
+val r = translate pb_constraintTheory.saturate_def;
+val r = translate pb_constraintTheory.weaken_aux_def;
+val r = translate pb_constraintTheory.weaken_def;
+
+val divide_side = Q.prove(
+  `∀x y. divide_side x y ⇔ y ≠ 0`,
+  Cases>>
+  EVAL_TAC>>
+  rw[EQ_IMP_THM]) |> update_precondition
+
+val r = translate check_polish_def;
+
+val r = translate FOLDL
+
+val r = translate check_pbpstep_def;
+val r = translate check_pbpsteps_def;
+
+Definition result_string_def:
+  (result_string Fail = INL (strlit "Proof checking failed\n")) ∧
+  (result_string (Cont _ _) = INL (strlit "Proof checking succeeded but derive contradiction\n")) ∧
+  (result_string Unsat = INR (strlit "Verified\n"))
+End
+
+val r = translate result_string_def;
+
+Definition check_pbp_def:
+  check_pbp pbf pbp =
+    let (id,fml) = build_fml 1 pbf LN in
+    result_string (check_pbpsteps pbp id fml)
+End
+
+val r = translate check_pbp_def;
+
+val check_unsat_2 = (append_prog o process_topdecs) `
+  fun check_unsat_2 f1 f2 =
+  case parse_pbf_full f1 of
+    Inl err => TextIO.output TextIO.stdErr err
+  | Inr fml =>
+  (case parse_pbp_full f2 of
+    Inl err => TextIO.output TextIO.stdErr err
+  | Inr pf =>
+    (case check_pbp fml pf of
+      Inl err => TextIO.output TextIO.stdErr err
+    | Inr succ => TextIO.print succ)
+  )`
+
+val check_unsat = (append_prog o process_topdecs) `
+  fun check_unsat u =
+  case CommandLine.arguments () of
+    [f1,f2] => check_unsat_2 f1 f2
+  | _ => TextIO.output TextIO.stdErr usage_string`
+
+(* TODO: Dummy spec *)
+val check_unsat_sem_def = Define`
+  check_unsat_sem cl fs err = fs`
+
+Theorem check_unsat_spec:
+   hasFreeFD fs
+   ⇒
+   app (p:'ffi ffi_proj) ^(fetch_v"check_unsat"(get_ml_prog_state()))
+     [Conv NONE []]
+     (COMMANDLINE cl * STDIO fs)
+     (POSTv uv. &UNIT_TYPE () uv *
+     COMMANDLINE cl * SEP_EXISTS err. STDIO (check_unsat_sem cl fs err))
+Proof
+  cheat
+QED
+
+Theorem check_unsat_whole_prog_spec2:
+   hasFreeFD fs ⇒
+   whole_prog_spec2 check_unsat_v cl fs NONE (λfs'. ∃err. fs' = check_unsat_sem cl fs err)
+Proof
+  rw[basis_ffiTheory.whole_prog_spec2_def]
+  \\ match_mp_tac (MP_CANON (DISCH_ALL (MATCH_MP app_wgframe (UNDISCH check_unsat_spec))))
+  \\ xsimpl
+  \\ rw[PULL_EXISTS]
+  \\ qexists_tac`check_unsat_sem cl fs x`
+  \\ qexists_tac`x`
+  \\ xsimpl
+  \\ rw[check_unsat_sem_def]
+  \\ every_case_tac
+  \\ simp[GSYM add_stdo_with_numchars,with_same_numchars]
+QED
+
+local
+
+val name = "check_unsat"
+val (sem_thm,prog_tm) =
+  whole_prog_thm (get_ml_prog_state()) name (UNDISCH check_unsat_whole_prog_spec2)
+val check_unsat_prog_def = Define`check_unsat_prog = ^prog_tm`;
+
+in
+
+Theorem check_unsat_semantics =
+  sem_thm
+  |> REWRITE_RULE[GSYM check_unsat_prog_def]
+  |> DISCH_ALL
+  |> SIMP_RULE(srw_ss())[GSYM CONJ_ASSOC,AND_IMP_INTRO];
+
+end
+
+val _ = export_theory();
