examples/pseudo_bool/pb_preconstraintScript.sml
@@ -1,0 +1,130 @@
+(*
+  Formalisation of (un-normalised) pseudo-boolean constraints
+*)
+
+open preamble;
+
+val _ = new_theory "pb_preconstraint";
+
+val _ = numLib.prefer_num();
+
+(* TODO: Possibly use mlstring, but need to check how it is supported in PBP *)
+Type var = “:num”
+
+Datatype:
+  lit = Pos var | Neg num
+End
+
+(*
+  Un-normalised pseudo-boolean constraints have the form:
+  c_i l_i ≥ n OR
+  c_i l_i = n OR
+  where coefficients c_i and n are arbitrary integers and l_i are literals
+*)
+Datatype:
+  pbc =
+    Equal ((int # lit) list) int
+  | GreaterEqual ((int # lit) list) int
+End
+
+(* integer-valued semantics *)
+
+Definition b2i_def[simp]:
+  b2i T = 1i ∧
+  b2i F = 0i
+End
+
+Definition eval_lit_def[simp]:
+  eval_lit w (Pos v) =     b2i (w v) ∧
+  eval_lit w (Neg v) = 1 - b2i (w v)
+End
+
+Definition eval_term_def[simp]:
+  eval_term w (c,l) = c * eval_lit w l
+End
+
+Definition iSUM_def:
+  (iSUM [] = 0:int) ∧
+  (iSUM (x::xs) = x + iSUM xs)
+End
+
+Definition eval_lhs_def[simp]:
+  eval_lhs w xs = iSUM (MAP (eval_term w) xs)
+End
+
+(* satisfaction of a pseudoboolean constraint *)
+Definition satisfies_pbc_def:
+  (satisfies_pbc w (Equal xs n) ⇔ eval_lhs w xs = n) ∧
+  (satisfies_pbc w (GreaterEqual xs n) ⇔ eval_lhs w xs ≥ n)
+End
+
+(* satisfaction of a set of pseudoboolean constraints *)
+Definition satisfies_def:
+  satisfies w pbf ⇔
+  ∀c. c ∈ pbf ⇒ satisfies_pbc w c
+End
+
+Definition satisfiable_def:
+  satisfiable pbf ⇔
+  ∃w. satisfies w pbf
+End
+
+Theorem satisfies_simp[simp]:
+  satisfies w EMPTY = T ∧
+  satisfies w (c INSERT f) = (satisfies_pbc w c ∧ satisfies w f) ∧
+  satisfies w (f ∪ h) = (satisfies w f ∧ satisfies w h)
+Proof
+  fs [satisfies_def] \\
+  metis_tac []
+QED
+
+(* Convert a list of pbc to one with ≥ constraints only *)
+Definition pbc_ge_def:
+  (pbc_ge (GreaterEqual xs n) = [GreaterEqual xs n]) ∧
+  (pbc_ge (Equal xs n) =
+    let xs' = MAP (λ(c:int,l). (-c,l)) xs in
+      [GreaterEqual xs' (-n) ; GreaterEqual xs n])
+End
+
+Theorem eq_disj:
+  (∀x. x = a ∨ x = b ⇒ P x) ⇔ P a ∧ P b
+Proof
+  metis_tac[]
+QED
+
+Theorem eval_term_negate:
+  ∀ls.
+  (MAP (eval_term w) (MAP (λ(c,l). (-c,l)) ls)) =
+  (MAP (\i. -i) (MAP (eval_term w) ls))
+Proof
+  Induct>>simp[]>>
+  Cases>>rw[eval_term_def]>>
+  intLib.ARITH_TAC
+QED
+
+Theorem iSUM_negate:
+  ∀ls. iSUM (MAP (\i. -i) ls) = -iSUM ls
+Proof
+  Induct>>simp[iSUM_def]>>
+  intLib.ARITH_TAC
+QED
+
+Theorem pbc_ge_thm:
+  ∀c.
+  satisfies w (set (pbc_ge c)) ⇔
+  satisfies_pbc w c
+Proof
+  Cases>>
+  simp[pbc_ge_def,satisfies_def]>>
+  rw[EQ_IMP_THM]
+  >- (
+    fs[satisfies_pbc_def,eq_disj,eval_term_negate,iSUM_negate]>>
+    intLib.ARITH_TAC)
+  >- (
+    fs[satisfies_pbc_def,eval_term_negate,iSUM_negate]>>
+    intLib.ARITH_TAC)>>
+  fs[satisfies_pbc_def]>>
+  intLib.ARITH_TAC
+QED
+
+val _ = export_theory();
