examples/pseudo_bool/README.md
@@ -1,7 +1,16 @@
 A checker for pseudo-boolean constraints
 
+[compilation](compilation):
+Compiling the pseudo-boolean constraints checker
+
+[pb_checkProgScript.sml](pb_checkProgScript.sml):
+This produces an executable program for pb_check
+
 [pb_checkScript.sml](pb_checkScript.sml):
 Pseudo-boolean constraints proof format and checker
 
 [pb_constraintScript.sml](pb_constraintScript.sml):
-A formalisation of pseudo-boolean constraints
+Formalisation of normalised pseudo-boolean constraints
+
+[pb_preconstraintScript.sml](pb_preconstraintScript.sml):
+Formalisation of (un-normalised) pseudo-boolean constraints
